Certainly! Let's prove that the XOR function cannot be represented by a linear model using algebraic equations.

### XOR Function Recap

The XOR function is defined as:

$$
\text{XOR}(x_1, x_2) = 
\begin{cases}
0 & \text{if } (x_1, x_2) = (0, 0) \\
1 & \text{if } (x_1, x_2) = (0, 1) \\
1 & \text{if } (x_1, x_2) = (1, 0) \\
0 & \text{if } (x_1, x_2) = (1, 1)
\end{cases}
$$

### Linear Model Assumption

Assume that we can represent the XOR function using a linear model of the form:

$$
f(\mathbf{x}) =
\begin{cases}
1 & \text{if } \mathbf{w}^T \mathbf{x} + b \geq 0 \\
0 & \text{if } \mathbf{w}^T \mathbf{x} + b < 0
\end{cases}
$$

where $\mathbf{w} = [w_1, w_2]^T$ are the weights, $b$ is the bias term, and $\mathbf{x} = [x_1, x_2]^T$ is the input vector.

This implies:

$$
f(\mathbf{x}) = \text{sign}(w_1 x_1 + w_2 x_2 + b)
$$

We want to check whether there exist values of $w_1$, $w_2$, and $b$ that satisfy the XOR function.

### Evaluating for Each Input Pair

We will evaluate $f(\mathbf{x})$ at the four input pairs and compare the results with the XOR function's outputs.

1. **For $(x_1, x_2) = (0, 0)$:**

$$
w_1 \cdot 0 + w_2 \cdot 0 + b = b
$$
Since XOR(0, 0) = 0, we require:

$$
b < 0
$$

2. **For $(x_1, x_2) = (0, 1)$:**

$$
w_1 \cdot 0 + w_2 \cdot 1 + b = w_2 + b
$$
Since XOR(0, 1) = 1, we require:

$$
w_2 + b \geq 0
$$
This implies:

$$
w_2 \geq -b \quad \text{(inequality 1)}
$$

3. **For $(x_1, x_2) = (1, 0)$:**

$$
w_1 \cdot 1 + w_2 \cdot 0 + b = w_1 + b
$$
Since XOR(1, 0) = 1, we require:

$$
w_1 + b \geq 0
$$
This implies:

$$
w_1 \geq -b \quad \text{(inequality 2)}
$$

4. **For $(x_1, x_2) = (1, 1)$:**

$$
w_1 \cdot 1 + w_2 \cdot 1 + b = w_1 + w_2 + b
$$
Since XOR(1, 1) = 0, we require:

$$
w_1 + w_2 + b < 0
$$
This implies:

$$
w_1 + w_2 < -b \quad \text{(inequality 3)}
$$

### Analyzing the Inequalities

We now have three inequalities derived from the XOR conditions:

1. $b < 0$
2. $w_2 \geq -b$
3. $w_1 \geq -b$
4. $w_1 + w_2 < -b$

Let's substitute the values of $w_1$ and $w_2$ from inequalities 1 and 2 into inequality 3:

Substituting $w_1 \geq -b$ and $w_2 \geq -b$ into $w_1 + w_2 < -b$, we get:

$$
(-b) + (-b) < -b
$$

$$
-2b < -b
$$

This simplifies to:

$$
-2b < -b \quad \text{or} \quad 2b > b
$$

Given that $b < 0$, the inequality $2b > b$ leads to a contradiction because for any negative $b$, $2b$ is more negative than $b$, not greater.

### Conclusion

This contradiction demonstrates that no real values of $w_1$, $w_2$, and $b$ can simultaneously satisfy the inequalities derived from the XOR function. Therefore, it is impossible to represent the XOR function using a linear model of the form $f(\mathbf{x}) = \text{sign}(w_1 x_1 + w_2 x_2 + b)$.

This algebraic approach, combined with the earlier geometric reasoning, shows that the XOR function cannot be implemented by a single linear threshold neuron.